---
sort: 6
---

# Comparison of Several MV Means

## Dreaming

### case 1: $$ \Sigma_1 = \Sigma_2 = \Sigma $$
이하 대부분은 벡터에 관한 이야기이다.



$$\bar X_i$$ estimates $$\mu_i$$, $$i=1,2$$.

$$S_p$$ estimates $$\Sigma$$, where $$S_p = \dfrac {(n_1 -1)S_1 + (n_2 - 1) S_2} {(n_1-1) + (n_2-1)} $$.

the test stats is, which is called **Hotelling's $$T^2$$**

$$

T^2 = \dfrac {n_1 n_2}{n_1 + n_2} \left( \bar {X_1 } - \bar {X_2} \right)^T S_p^{-1} \left( \bar {X_1 } - \bar {X_2} \right)

$$

where $$ \dfrac {(n_1 - 1) + (n_2 - 1) - (p - 1)} {p [ (n_1 - 1) + (n_2 - 1) ]} \; T^2 = \dfrac {n_1 + n_2  - p - 1} {p [ (n_1 + n_2 - 2) ]} \; T^2 \overset{H_0}{\sim} F_{p, n_1 + n_2 -p  - 1}$$. (p.285 for pf)



**CR for $$\mu_1 - \mu_2$$** will be

$$

Pr \left[ 
\left( 
\left( 
(\bar X_1 - \bar X_2 ) - (\mu_1 - \mu_2) 
\right)^T
\left( 
\left( 
\dfrac {1}{n_1} + \dfrac {1}{n_2}
\right) S_p

\right)^{-1}

\left( 
(\bar X_1 - \bar X_2 ) - (\mu_1 - \mu_2) 
\right)

\le c^2

\right)
\right] = 1-\alpha

$$

where $$ c^2= \dfrac {p [ (n_1 + n_2 - 2) ]} {n_1 + n_2  - p - 1}  \; T^2 \overset{H_0}{\sim} F_{p, n_1 + n_2 -p  - 1} (\alpha)$$. 
* 이때 constant가 역수가 되었음을 눈치.
* The equality will define the boundary of a region.
* The region is an ellipsoid centered at $$(\bar X_1 - \bar X_2)$$.

#### Example) Testing $$H_0 : \mu_1 - \mu_2 = 0$$ at $$\alpha=0.05$$ is equivalent to see whether falls within the confidence region

- Axes of the confidence region
		* let $$\lambda_1 , \cdots, \lambda_p$$ are ev of $$S_p$$.
		* let $$e_1 , \cdots, e_p$$ are evc of $$S_p$$.
	* then $$e_i$$'s are the direction of CI
	* $$\sqrt{\lambda_i} \sqrt{ \left( \dfrac{1}{n_1} + \dfrac{1}{n_2}\right) c^2} $$are the half-length of the CR [Link]()

let $$ c^2= \dfrac {p [ (n_1 + n_2 - 2) ]} {n_1 + n_2  - p - 1}  \; T^2 \overset{H_0}{\sim} F_{p, n_1 + n_2 -p  - 1} (\alpha)$$.

then $$100(1-\alpha)%$$ **simultaneous CI** for $$a'(\mu_1 - \mu_2)$$ for all $$a$$ is $$ a' \left( \bar X_1 - \bar X_2 \right) \pm c \sqrt{a' \left( \dfrac{1}{n_1} + \dfrac{1}{n_2}\right) S_p a} $$



#### Example) simultaneous CI for $$(\mu_{1i} - \mu_{2i}), i=1, \cdots, p$$.

let $$a' = \left[0, \cdots, 0, 1, 0, \cdots, 0 \right]$$. 이때 $$a'$$가 하나만 1이고 나머지 0이면, 어떤 특별한 한 axis로 proj하라는 의미. [link]()

let $$\mu_1 - \mu_2 = \left[ \mu_{1i} - \mu_{2i} \right]_{i=1,\cdots,p}$$.

$$ a'(\bar X_1 - \bar X_2) = \bar X_{1i} - \bar X_{2i}$$, $$a' \left( \dfrac {1}{n_1} + \dfrac {1}{n_2} \right) S_p a = \left( \dfrac {1}{n_1} + \dfrac {1}{n_2} \right) S_{p \; ii}$$
* $$S_{p \; ii}$$ : p번째 변수의 표본 cov. 이는 단변량에서 나왔던 공통 cov, 즉 샘플 se와 표기법이 동일해지며 유사하다. (ch1) [link]()

the Bonferroni's $$100(1-\alpha)\% $$ simultaneous CI for $$(\mu_{1i} - \mu_{2i})$$ is $$ (\bar X_1 - \bar X_2) \pm t_{n_2 + n_2 -2, (\dfrac{\alpha}{2p})} \sqrt{\left( \dfrac {1}{n_1} + \dfrac {1}{n_2} \right) S_{p \; ii}}$$.


### case 2: $$ \Sigma_1 \not = \Sigma_2 $$

assume $$n_1 - p , \; n_2 - p$$ are large. 

for $$H_0 : \mu_1 - \mu_2 = 0$$, test stat becomes $$T^2 = (\bar X_1 - \bar X_2 )' \left[ \dfrac{1}{n_1} S_1 + \dfrac {1}{n_2} S_2 \right]^{-1} (\bar X_1 - \bar X_2 ) \overset{H_0}{\sim} \chi_p^2$$.



```note

$$
E(\bar X_1 - \bar X_2 ) = \mu_1 - \mu_2
$$

$$
Cov(\bar X_1 - \bar X_2 ) = Cov(\bar X_1) + Cov(\bar X_2 ) - 2 Cov(\bar X_1, \bar X_2 ) = \dfrac{1}{n_1} \Sigma_1 + \dfrac {1}{n_2} \Sigma_2 - 0
$$


$$
\bar X_1 - \bar X_2 \overset{\cdot}{\sim} N_p \left( \mu_1 - \mu_2, \dfrac{1}{n_1} \Sigma_1 + \dfrac {1}{n_2} \Sigma_2  \right)
\tag{∵ CLT}
$$

$$\\[3ex]
$$

$$
\text{under } H_0, 
$$

$$
S_1 \overset{p}{\to} \Sigma_1, S_2 \overset{p}{\to} \Sigma_2 \tag{∵ WLLN}
$$

$$
(\bar X_1 - \bar X_2 )' \left[ \dfrac{1}{n_1} S_1 + \dfrac {1}{n_2} S_2\right]^-1 (\bar X_1 - \bar X_2 ) \overset{app}{\sim} \chi_p^2 \tag{∵ Slutsky's thm}
$$
```



***why Cov become 0???***

i.e. reject $$H_0$$ if $$T^2 > \chi_p^2 (\alpha)$$.

CI becomes 

$$

Pr \left[ 
\left( 
\left( 
(\bar X_1 - \bar X_2 ) - (\mu_1 - \mu_2) 
\right)^T
\left( 
\left( 
\dfrac {1}{n_1} + \dfrac {1}{n_2}
\right) S_2

\right)^{-1}

\left( 
(\bar X_1 - \bar X_2 ) - (\mu_1 - \mu_2) 
\right)

\le \chi_p^2

\right)
\right] = 1-\alpha

$$

차이는~~


Remark: if $$n_1 = n_2 = 2$$,



----------------------------------

